\section{Equivalent Cauchy sequences}\label{sec 5.2}

\begin{definition}[\(\varepsilon\)-close sequences]\label{5.2.1}
    Let \((a_n)_{n = 0}^{\infty}\) and \((b_n)_{n = 0}^{\infty}\) be two sequences, and let \(\varepsilon > 0\).
    We say that the sequence \((a_n)_{n = 0}^{\infty}\) is \emph{\(\varepsilon\)-close} to \((b_n)_{n = 0}^{\infty}\) iff \(a_n\) is \(\varepsilon\)-close to \(b_n\) for each \(n \in \mathbf{N}\).
    In other words, the sequence \(a_0, a_1, a_2, \dots\) is \(\varepsilon\)-close to the sequence \(b_0, b_1, b_2, \dots\) iff \(\abs*{a_n - b_n} \leq \varepsilon\) for all \(n = 0, 1, 2, \dots\).
\end{definition}

\setcounter{theorem}{2}
\begin{definition}[\(Eventually \varepsilon\)-close sequences]\label{5.2.3}
    Let \((a_n)_{n = 0}^{\infty}\) and \((b_n)_{n = 0}^{\infty}\) be two sequences, and let \(\varepsilon > 0\).
    We say that the sequence \((a_n)_{n = 0}^{\infty}\) is \emph{eventually \(\varepsilon\)-close} to \((b_n)_{n = 0}^{\infty}\) iff there exists an \(N \geq 0\) such that the sequences \((a_n)_{n = N}^{\infty}\) and \((b_n)_{n = N}^{\infty}\) are \(\varepsilon\)-close.
    In other words, \(a_0, a_1, a_2, \dots\) is eventually \(\varepsilon\)-close to \(b_0, b_1, b_2, \dots\) iff there exists an \(N \geq 0\) such that \(\abs*{a_n - b_n} \leq \varepsilon\) for all \(n \geq N\).
\end{definition}

\begin{remark}\label{5.2.4}
    Again, the notations for \(\varepsilon\)-close sequences and eventually \(\varepsilon\)-close sequences are not standard in the literature, and we will not use them outside of this section.
\end{remark}

\setcounter{theorem}{5}
\begin{definition}[Equivalent sequences]\label{5.2.6}
    Two sequences \((a_n)_{n = 0}^{\infty}\) and \((b_n)_{n = 0}^{\infty}\) are \emph{equivalent} iff for each rational \(\varepsilon > 0\), the sequences \((a_n)_{n = 0}^{\infty}\) and \((b_n)_{n = 0}^{\infty}\) are eventually \(\varepsilon\)-close.
    In other words, \(a_0, a_1, a_2, \dots\) and \(b_0, b_1, b_2, \dots\) are equivalent iff for every rational \(\varepsilon > 0\), there exists an \(N \geq 0\) such that \(\abs*{a_n - b_n} \leq \varepsilon\) for all \(n \geq N\).
\end{definition}

\begin{remark}\label{5.2.7}
    As with Definition \ref{5.1.8}, the quantity \(\varepsilon > 0\) is currently restricted to be a positive rational, rather than a positive real.
    However, we shall eventually see that it makes no difference whether \(\varepsilon\) ranges over the positive rationals or positive reals.
\end{remark}

\begin{additional corollary}\label{ac 5.2.1}
Equivalence defined as Definition \ref{5.2.6} is reflexive, symmetric and transitive.
\end{additional corollary}

\begin{proof}
    Let \((a_n)_{n = m}^\infty\), \((b_n)_{n = m}^\infty\), \((c_n)_{n = m}^\infty\) be sequences of rationals.
    We have
    \begin{align*}
                 & \forall\ \varepsilon \in \mathbf{Q}^+, \forall\ n \geq m, \abs*{a_n - a_n} = \abs*{0} = 0 \leq \varepsilon                                      \\
        \implies & (a_n)_{n = m}^\infty = (a_n)_{n = m}^\infty                                                                & \text{(by Definition \ref{5.2.6})}
    \end{align*}
    and thus Definition \ref{5.2.6} is reflexive.

    Now suppose that \((a_n)_{n = m}^\infty = (b_n)_{n = m}^\infty\).
    Then we have
    \begin{align*}
                 & (a_n)_{n = m}^\infty = (b_n)_{n = m}^\infty                                                                               \\
        \implies & \forall\ \varepsilon \in \mathbf{Q}^+, \exists\ N \in \mathbf{N} \land N \geq m:                                          \\
                 & \forall\ n \geq N, \abs*{a_n - b_n} \leq \varepsilon                             & \text{(by Definition \ref{5.2.6})}     \\
        \implies & \forall\ \varepsilon \in \mathbf{Q}^+, \exists\ N \in \mathbf{N} \land N \geq m:                                          \\
                 & \forall\ n \geq N, \abs*{b_n - a_n} \leq \varepsilon                             & \text{(by Proposition \ref{4.3.3}(f))} \\
        \implies & (b_n)_{n = m}^\infty = (a_n)_{n = m}^\infty                                      & \text{(by Definition \ref{5.2.6})}
    \end{align*}
    and thus Definition \ref{5.2.6} is symmetric.

    Finally suppose that \((a_n)_{n = m}^\infty = (b_n)_{n = m}^\infty\) and \((b_n)_{n = m}^\infty = (c_n)_{n = m}^\infty\).
    Then we have
    \begin{align*}
                 & \big((a_n)_{n = m}^\infty = (b_n)_{n = m}^\infty\big) \land \big((b_n)_{n = m}^\infty = (c_n)_{n = m}^\infty\big)                                                \\
        \implies & \forall\ \varepsilon \in \mathbf{Q}^+, \exists\ N_1, N_2 \in \mathbf{N} \land N_1, N_2 \geq m:                       & \text{(by Definition \ref{5.2.6})}        \\
                 & \begin{cases}
            \abs*{a_n - b_n} \leq \frac{\varepsilon}{2} & \forall\ n \geq N_1 \\
            \abs*{b_n - c_n} \leq \frac{\varepsilon}{2} & \forall\ n \geq N_2 \\
        \end{cases}                                                                                                                                        \\
        \implies & \forall\ \varepsilon \in \mathbf{Q}^+, \exists\ N = \max(N_1, N_2) \geq m:                                           & \text{(by Proposition \ref{2.2.13})}      \\
                 & \forall\ n \geq N, (\abs*{a_n - b_n} \leq \frac{\varepsilon}{2}) \land (\abs*{b_n - c_n} \leq \frac{\varepsilon}{2})                                             \\
        \implies & \forall\ \varepsilon \in \mathbf{Q}^+, \exists\ N = \max(N_1, N_2) \geq m:                                                                                       \\
                 & \forall\ n \geq N, \abs*{a_n - b_n} + \abs*{b_n - c_n} \leq \varepsilon                                              & \text{(by Proposition \ref{4.2.9}(c)(d))} \\
        \implies & \forall\ \varepsilon \in \mathbf{Q}^+, \exists\ N = \max(N_1, N_2) \geq m:                                                                                       \\
                 & \forall\ n \geq N, \abs*{a_n - c_n} \leq \abs*{a_n - b_n} + \abs*{b_n - c_n} \leq \varepsilon                        & \text{(by Proposition \ref{4.3.3}(b))}    \\
        \implies & (a_n)_{n = m}^\infty = (c_n)_{n = m}^\infty                                                                          & \text{(by Definition \ref{5.2.6})}
    \end{align*}
    and thus Definition \ref{5.2.6} is transitive.
\end{proof}

\begin{proposition}\label{5.2.8}
    Let \((a_n)_{n = 1}^{\infty}\) and \((b_n)_{n = 1}^{\infty}\) be the sequences \(a_n = 1 + 10^{-n}\) and \(b_n = 1 - 10^{-n}\).
    Then the sequences \(a_n, b_n\) are equivalent.
\end{proposition}

\begin{proof}
    We need to prove that for every \(\varepsilon > 0\), the two sequences \((a_n)_{n = 1}^{\infty}\) and \((b_n)_{n = 1}^{\infty}\) are eventually \(\varepsilon\)-close to each other.
    So we fix an \(\varepsilon > 0\).
    We need to find an \(N > 0\) such that \((a_n)_{n = 1}^{\infty}\) and \((b_n)_{n = 1}^{\infty}\) are \(\varepsilon\)-close;
    in other words, we need to find an \(N > 0\) such that
    \[
        \abs*{a_n - b_n} \leq \varepsilon \text{ for all } n \geq N.
    \]
    However, we have
    \[
        \abs*{a_n - b_n} = \abs*{(1 + 10^{-n}) - (1 - 10^{-n})} = 2 \times 10^{-n}.
    \]
    Since \(10^{-n}\) is a decreasing function of \(n\) (i.e., \(10^{-m} < 10^{-n}\) whenever \(m > n\);
    this is easily proven by induction), and \(n \geq N\), we have \(2 \times 10^{-n} \leq 2 \times 10^{-N}\).
    Thus we have
    \[
        \abs*{a_n - b_n} \leq 2 \times 10^{-N} \text{ for all } n \geq N.
    \]
    Thus in order to obtain \(\abs*{a_n - b_n} \leq \varepsilon\) for all \(n \geq N\), it will be sufficient to choose \(N\) so that \(2 \times 10^{-N} \leq \varepsilon\).
    This is easy to do using logarithms, but we have not yet developed logarithms yet, so we will use a cruder method.
    First, we observe \(10^N\) is always greater than \(N\) for any \(N \geq 1\) (see Exercise \ref{ex 4.3.5}).
    Thus \(10^{-N} \leq 1 / N\), and so \(2 \times 10^{-N} \leq 2 / N\).
    Thus to get \(2 \times 10^{-N} \leq \varepsilon\), it will suffice to choose \(N\) so that \(2 / N \leq \varepsilon\), or equivalently that \(N \geq 2 / \varepsilon\).
    But by Proposition \ref{4.4.1} we can always choose such an \(N\), and the claim follows.
\end{proof}

\begin{remark}\label{5.2.9}
    Proposition \ref{5.2.8}, in decimal notation, asserts that
    \[
        1.0000 \dots = 0.9999 \dots.
    \]
\end{remark}

\exercisesection

\begin{exercise}\label{ex 5.2.1}
    Show that if \((a_n)_{n = 1}^{\infty}\) and \((b_n)_{n = 1}^{\infty}\) are equivalent sequences of rationals, then \((a_n)_{n = 1}^{\infty}\) is a Cauchy sequence if and only if \((b_n)_{n = 1}^{\infty}\) is a Cauchy sequence.
\end{exercise}

\begin{proof}
    Let \(j, k \in \mathbf{Z}^+\).
    Since \((a_n)_{n = 1}^\infty = (b_n)_{n = 1}^\infty\), by Definition \ref{5.2.6} we have
    \[
        \forall\ \varepsilon \in \mathbf{Q}^+, \exists\ N_1 \in \mathbf{Z}^+ : \forall\ n \geq N_1, \abs*{a_n - b_n} \leq \frac{\varepsilon}{3}.
    \]
    Then we have
    \begin{align*}
                 & (a_n)_{n = 1}^\infty \text{ is a Cauchy sequence}                                                                                    \\
        \implies & \exists\ N_2 \in \mathbf{Z}^+ : \forall\ j, k \geq N,                                                                                \\
                 & \abs*{a_j - a_k} \leq \frac{\varepsilon}{3}                                              & \text{(by Definition \ref{5.1.8})}        \\
        \implies & \exists\ N = \max(N_1, N_2) \in \mathbf{Z}^+ : \forall\ j, k \geq N,                     & \text{(by Proposition \ref{2.2.13})}      \\
                 & \abs*{a_j - a_k} \leq \frac{\varepsilon}{3}                                                                                          \\
        \implies & \exists\ N = \max(N_1, N_2) \in \mathbf{Z}^+ : \forall\ j, k \geq N,                                                                 \\
                 & \abs*{a_j - a_k} + \abs*{a_j - b_j} + \abs*{a_k - b_k}                                                                               \\
                 & \leq \frac{\varepsilon}{3} + \frac{\varepsilon}{3} + \frac{\varepsilon}{3} = \varepsilon & \text{(by Proposition \ref{4.2.9}(c)(d))} \\
        \implies & \exists\ N = \max(N_1, N_2) \in \mathbf{Z}^+ : \forall\ j, k \geq N,                                                                 \\
                 & \abs*{a_j - a_k} + \abs*{b_j - a_j} + \abs*{a_k - b_k} \leq \varepsilon                  & \text{(by Proposition \ref{4.3.3}(f))}    \\
        \implies & \exists\ N = \max(N_1, N_2) \in \mathbf{Z}^+ : \forall\ j, k \geq N,                                                                 \\
                 & \abs*{b_j - b_k} = \abs*{a_j - a_k + b_j - a_j + a_k - b_k}                                                                          \\
                 & \leq \abs*{a_j - a_k} + \abs*{b_j - a_j} + \abs*{a_k - b_k} \leq \varepsilon             & \text{(by Proposition \ref{4.3.3}(b))}    \\
        \implies & (b_n)_{n = 1}^\infty \text{ is a Cauchy sequence}.                                       & \text{(by Definition \ref{5.1.8})}
    \end{align*}
    Using similar arguments we can show that \((b_n)_{n = 1}^\infty\) is a Cauchy sequence implies \((a_n)_{n = 1}^\infty\) is a Cauchy sequence.
    Thus we conclude that \((a_n)_{n = 1}^\infty\) is a Cauchy sequence iff \((b_n)_{n = 1}^\infty\) is a Cauchy sequence.
\end{proof}

\begin{exercise}\label{ex 5.2.2}
    Let \(\varepsilon > 0\).
    Show that if \((a_n)_{n = 1}^{\infty}\) and \((b_n)_{n = 1}^{\infty}\) are eventually \(\varepsilon\)-close, then \((a_n)_{n = 1}^{\infty}\) is bounded if and only if \((b_n)_{n = 1}^{\infty}\) is bounded.
\end{exercise}

\begin{proof}
    Since \((a_n)_{n = 1}^{\infty}\) and \((b_n)_{n = 1}^{\infty}\) are eventually \(\varepsilon\)-close, by Definition \ref{5.2.3} we have
    \[
        \exists\ N \in \mathbf{Z}^+ : \forall\ n \geq N, \abs*{a_n - b_n} \leq \varepsilon.
    \]
    Then we have
    \begin{align*}
                 & (a_n)_{n = 1}^\infty \text{ is bounded}                                                                                                                    \\
        \implies & \exists\ M \in \mathbf{Q} \setminus \mathbf{Q}^- : \forall\ n \geq 1, \abs*{a_n} \leq M                        & \text{(by Definition \ref{5.1.12})}       \\
        \implies & \exists\ M \in \mathbf{Q} \setminus \mathbf{Q}^- : \forall\ n \geq \max(1, N), \abs*{a_n} \leq M               & \text{(by Proposition \ref{2.2.13})}      \\
        \implies & \exists\ M \in \mathbf{Q} \setminus \mathbf{Q}^- : \forall\ n \geq \max(1, N), \abs*{-a_n} \leq M              & \text{(by Proposition \ref{4.3.3}(d))}    \\
        \implies & \exists\ M \in \mathbf{Q} \setminus \mathbf{Q}^- : \forall\ n \geq \max(1, N),                                                                             \\
                 & \abs*{-a_n} + \abs*{a_n - b_n} \leq M + \varepsilon                                                            & \text{(by Proposition \ref{4.2.9}(c)(d))} \\
        \implies & \exists\ M \in \mathbf{Q} \setminus \mathbf{Q}^- : \forall\ n \geq \max(1, N),                                                                             \\
                 & \abs*{-a_n + a_n - b_n} \leq \abs*{-a_n} + \abs*{a_n - b_n} \leq M + \varepsilon                               & \text{(by Proposition \ref{4.3.3}(b))}    \\
        \implies & \exists\ M \in \mathbf{Q} \setminus \mathbf{Q}^- : \forall\ n \geq \max(1, N),                                                                             \\
                 & \abs*{-b_n} \leq M + \varepsilon                                                                               & \text{(by Proposition \ref{4.2.4})}       \\
        \implies & \exists\ M \in \mathbf{Q} \setminus \mathbf{Q}^- : \forall\ n \geq \max(1, N), \abs*{b_n} \leq M + \varepsilon & \text{(by Proposition \ref{4.3.3}(d))}    \\
        \implies & \exists\ M \in \mathbf{Q} \setminus \mathbf{Q}^- : \forall\ n \geq 1,                                                                                      \\
                 & \abs*{b_n} \leq M + \varepsilon + \max_{1 \leq n \leq N - 1}\{\abs*{b_n}\}                                     & \text{(by Lemma \ref{5.1.14})}            \\
        \implies & (a_n)_{n = 1}^\infty \text{ is bounded}.                                                                       & \text{(by Definition \ref{5.1.12})}
    \end{align*}
    Using similar arguments we can show that \((b_n)_{n = 1}^\infty\) is bounded implies \((a_n)_{n = 1}^\infty\) is bounded.
    Thus we conclude that \((a_n)_{n = 1}^\infty\) is bounded iff \((b_n)_{n = 1}^\infty\) is bounded.
\end{proof}