\section{Some standard limits}\label{sec 6.5}

\begin{additional corollary}\label{ac 6.5.1}
We have
\[
    \lim_{n \to \infty} c = c
\]
for any constant \(c\).
\end{additional corollary}

\begin{proof}
    Let \((a_n)_{n = 1}^\infty\) be a constant sequence where \(a_n = c\) for all \(n \geq 1\), and let \(N \in \mathbf{N}\).
    Then \(\forall \varepsilon \in \mathbf{R}^+\), \(\exists\ N \geq 1\) such that for every \(n \geq N\),
    \[
        \abs*{a_n - c} = \abs*{c - c} = 0 \leq \varepsilon.
    \]
    Thus by Definition \ref{6.1.8} we have \(\lim_{n \to \infty} a_n = \lim_{n \to \infty} c = c\).
\end{proof}

\begin{corollary}\label{6.5.1}
    We have \(\lim_{n \to \infty} 1 / n^{1 / k} = 0\) for every integer \(k \geq 1\).
\end{corollary}

\begin{proof}
    From Lemma \ref{5.6.6} we know that \(1 / n^{1 / k}\) is a decreasing function of \(n\), while being bounded below by \(0\).
    By Additional Corollary \ref{ac 6.3.1} (for decreasing sequences instead of increasing sequences) we thus know that this sequence converges to some limit \(L \geq 0\):
    \[
        L = \lim_{n \to \infty} 1 / n^{1 / k}.
    \]
    Raising this to the \(k^{th}\) power and using the limit laws (or more precisely, Theorem \ref{6.1.19}(b) and induction), we obtain
    \[
        L^k = \lim_{n \to \infty} 1 / n.
    \]
    By Proposition \ref{6.1.11} we thus have \(L^k = 0\);
    but this means that \(L\) cannot be positive (else \(L^k\) would be positive), so \(L = 0\), and we are done.
\end{proof}

\begin{lemma}\label{6.5.2}
    Let \(x\) be a real number.
    Then the limit \(\lim_{n \to \infty} x^n\) exists and is equal to zero when \(\abs*{x} < 1\), exists and is equal to \(1\) when \(x = 1\), and diverges when \(x = -1\) or when \(\abs*{x} > 1\).
\end{lemma}

\begin{proof}
    We first show that if \(\abs*{x} < 1\), then \(\lim_{n \to \infty} x^n = 0\).
    Since \(0 \leq \abs*{x} < 1\), we have
    \begin{align*}
                 & 0 \leq \abs*{x} < 1                                                                           \\
        \implies & \lim_{n \to \infty} \abs*{x}^n = 0                     & \text{(by Proposition \ref{6.3.10})} \\
        \implies & (-1)\lim_{n \to \infty} \abs*{x}^n = (-1) \times 0 = 0                                        \\
        \implies & \lim_{n \to \infty} -\abs*{x}^n = 0.                   & \text{(by Theorem \ref{6.1.19})}
    \end{align*}
    So \(\lim_{n \to \infty} -\abs*{x}^n = \lim_{n \to \infty} \abs*{x}^n\).
    And because \(-\abs*{x}^n \leq x^n \leq \abs*{x}^n\), by Squeeze test (Corollary \ref{6.4.14}) we have \(\lim_{n \to \infty} x^n = 0\).

    Next we show that if \(x = 1\), then \(\lim_{n \to \infty} x^n = 1\).
    This is done by Additional Corollary \ref{ac 6.5.1}.

    Finally we show that if \(x = -1\) or \(\abs*{x} > 1\), then \(\lim_{n \to \infty} x^n\) does not exist.
    If \(x = -1\), then we have sequence \(-1, 1, -1, 1, \dots\), which is not eventually \(1\)-steady for any \(n \geq 1\) and thus does not converge to any value.
    If \(\abs*{x} > 1\), then we can divide into two cases:
    \begin{itemize}
        \item If \(x > 1\), then by Exercise \ref{ex 6.3.4} \(\lim_{n \to \infty} x^n\) does not exist.
        \item If \(x < -1\), then \(\forall n \geq 1\) we have
              \begin{align*}
                  \abs*{x^{n + 1} - x^n} & = \abs*{x^n(x - 1)}      \\
                                         & = \abs*{x^n}\abs*{x - 1} \\
                                         & > \abs*{x^n}\abs*{-2}    \\
                                         & = 2\abs*{x^n}            \\
                                         & > 2.
              \end{align*}
              This means \(x\) is not a Cauchy sequence, so by Theorem \ref{6.4.18} \(\lim_{n \to \infty} x^n\) does not exist.
    \end{itemize}
    From all cases above we conclude that if \(\abs*{x} > 1\) then \(\lim_{n \to \infty} x^n\) does not exist.
\end{proof}

\begin{lemma}\label{6.5.3}
    For any \(x > 0\), we have \(\lim_{n \to \infty} x^{1 / n} = 1\).
\end{lemma}

\begin{proof}
    We first show that \(\forall \varepsilon, M \in \mathbf{R}^+\), \(\exists\ n \geq 1\) such that \(M^{1 / n} \leq 1 + \varepsilon\).
    Since \(1 / (1 + \varepsilon) < 1\), by Lemma \ref{6.5.2} we have \(\lim_{n \to \infty} 1 / (1 + \varepsilon)^n = 0\).
    Let \(a_n = 1 / (1 + \varepsilon)^n\).
    Then \(\inf(a_n)_{n = 1}^\infty = 0\).
    Since \(1 / M > 0\), we have \(1 / M > \inf(a_n)_{n = 1}^\infty\).
    By Remark \ref{6.3.7} \(\exists\ n \geq 1\) such that \(a_n = 1 / (1 + \varepsilon)^n < 1 / M\).
    Thus we have \(M < (1 + \varepsilon)^n\), and by Proposition \ref{5.6.9}(d) \(M^{1 / n} < 1 + \varepsilon\).

    Now we show that \(\lim_{n \to \infty} x^{1 / n} = 1\).
    We split into two cases:
    \begin{itemize}
        \item If \(x \geq 1\), then by the proof above we have \(\forall \varepsilon \in \mathbf{R}^+\), \(\exists\ n \geq 1\) such that \(x^{1 / n} < 1 + \varepsilon\).
              Thus
              \begin{align*}
                           & x \geq 1                                                                                 \\
                  \implies & x^{1 / n} \geq 1^{1 / n} = 1                       & \text{(by Lemma \ref{5.6.6}(d)(e))} \\
                  \implies & \abs*{x^{1 / n} - 1} = x^{1 / n} - 1 < \varepsilon
              \end{align*}
              and by Definition \ref{6.1.8} \(\lim_{n \to \infty} x^{1 / n} = 1\).
        \item If \(x < 1\), then \(1 / x > 1\).
              So from the proof above we have \(\lim_{n \to \infty} x^{-1 / n} = 1\).
              By Theorem \ref{6.1.19}(e) we have \(\lim_{n \to \infty} x^{-1 / n} = (\lim_{n \to \infty} x^{1 / n})^{-1} = 1^{-1} = 1\).
    \end{itemize}
    From all cases above we conclude that \(\lim_{n \to \infty} x^{1 / n} = 1\).
\end{proof}

\exercisesection

\begin{exercise}\label{ex 6.5.1}
    Show that \(\lim_{n \to \infty} 1 / n^q = 0\) for any rational \(q > 0\).
    Conclude that the limit \(\lim_{n \to \infty} n^q\) does not exist.
\end{exercise}

\begin{proof}
    We firs show that \(\lim_{n \to \infty} 1 / n^q = 0\) for every \(q \in \mathbf{Q}^+\).
    Let \(q = a / b\) where \(a, b \in \mathbf{Z}^+\).
    Then we have
    \begin{align*}
                 & \frac{1}{n^q} = \frac{1}{n^{a / b}} = \bigg(\frac{1}{n^{1 / b}}\bigg)^a                                       \\
        \implies & \lim_{n \to \infty} 1 / n^{1 / b} = 0                                   & \text{(by Corollary \ref{6.5.1})}   \\
        \implies & \lim_{n \to \infty} (1 / n^{1 / b})^a = 0                               & \text{(by Theorem \ref{6.1.19}(b))} \\
        \implies & \lim_{n \to \infty} 1 / n^q = 0.                                        & \text{(by Definition \ref{5.6.7})}
    \end{align*}

    Now we show that \(\lim_{n \to \infty} n^q\) does not exist.
    Suppose for sake of contradiction that \(\lim_{n \to \infty} n^q\) exists and equals to \(y\).
    Since \(n \geq 1\), we have \(n^q \geq 1\), so \(y \geq 1\).
    Then we have
    \begin{align*}
                 & (\lim_{n \to \infty} n^q)^{-1} = y^{-1}    & \text{(by Theorem \ref{6.1.19}(e))} \\
        \implies & \lim_{n \to \infty} (n^q)^{-1} = y^{-1}    & \text{(by Theorem \ref{6.1.19}(e))} \\
        \implies & \lim_{n \to \infty} \frac{1}{n^q} = y^{-1}                                       \\
        \implies & y^{-1} = 0.                                & \text{(by proof above)}
    \end{align*}
    But this means \(y = 1 / 0\), which means such \(y\) does not exist, a contradiction.
    Thus \(\lim_{n \to \infty} n^q\) does not exist.
\end{proof}

\begin{exercise}\label{ex 6.5.2}
    Prove Lemma \ref{6.5.2}.
\end{exercise}

\begin{proof}
    See Lemma \ref{6.5.2}.
\end{proof}

\begin{exercise}\label{ex 6.5.3}
    Prove Lemma \ref{6.5.3}.
\end{exercise}

\begin{proof}
    See Lemma \ref{6.5.3}.
\end{proof}